sketched proofs of local reasoning

unitb/decomposition/component.lean
@@ -1,7 +1,7 @@
 
 import unitb.models.nondet
 
-namespace d
+namespace decomposition
 
 open nondet unitb function
 
@@ -12,16 +12,17 @@ parameter α : Type
 @[reducible]
 private def pred := α → Prop
 
-parameter {α}
-
 structure program : Type 2 :=
   (asm : α → α → Prop)
   (mch : nondet.program α)
+
+parameter {α}
 
 def compatible {t : Type} (m : t → program) : Prop :=
 ∀ i j, i ≠ j → ∀ s s', is_step (m i).mch s s' → (m i).asm s s'
 
 def compose {t : Type} (m : t → program) {s₀ : α}
+  (hasm : α → α → Prop)
   (h₀ : ∀ i, (m i).mch.first s₀)
   (h : compatible m)
 : program :=
@@ -31,7 +32,7 @@ def compose {t : Type} (m : t → program) {s₀ : α}
     , first := λ s, ∀ i, (m i).mch.first s
     , first_fis := ⟨_,h₀⟩
     , event' := λ i, (m i.1).mch.event' i.2 }
-, asm := sorry }
+, asm := hasm }
 
 def step (p : program) (s s' : α) : Prop :=
 nondet.is_step p.mch s s' ∨ p.asm s s'
@@ -53,7 +54,7 @@ lemma ex_of_ex_mch (s : program) (τ : stream α)
   (h : s.mch.ex τ)
 : s.ex τ :=
 begin
-  apply d.program.ex.mk,
+  apply decomposition.program.ex.mk,
   { apply h.init },
   { unfold saf_ex,
     apply temporal.henceforth_entails_henceforth _ _ h.safety,
@@ -69,9 +70,9 @@ instance : system_sem program :=
   ex := λ p, program.ex p
 , init_sem  := λ s p τ Hτ H₀, by { apply H₀, apply Hτ.init }
 , inhabited := λ s, exists_imp_exists (ex_of_ex_mch s) (system_sem.inhabited s.mch)
-, safety    := λ s p, d.program.ex.safety
+, safety    := λ s p, decomposition.program.ex.safety
 , transient_sem := λ s p q τ Hτ T, by apply transient.semantics' _ Hτ.liveness T }
 
 end
 
-end d
+end decomposition
