unitb/decomposition/lemmas.lean
@@ -1,0 +1,73 @@
+
+import unitb.decomposition.component
+
+universe variables u
+
+namespace decomposition
+section
+
+open predicate unitb function
+
+parameter {α  : Type}
+parameter {t : Type}
+parameter s : t → program α
+parameter {s₀ : α}
+parameter {asm : α → α → Prop}
+parameter {h₀ : ∀ i, (s i).mch.first s₀}
+parameter {h : compatible s}
+def s' := compose s asm h₀ h
+
+variables {i : t}
+variables {p q : pred' α}
+
+lemma local_reasoning.transient
+  (T : transient' (s i) p q)
+: transient' s' p q :=
+begin
+  unfold transient' system.transient nondet.program.transient comp,
+  unfold transient' system.transient nondet.program.transient comp at T,
+  cases T with e Te,
+  cases e,
+  case some e
+  { existsi some (⟨i,e⟩ : Σ i, (s i).mch.lbl),
+    unfold s' compose program.mch nondet.program.lbl,
+    apply nondet.program.falsify.mk,
+    { apply Te.enable },
+    { apply Te.schedule },
+    { apply Te.negate' } },
+  case none
+  { existsi none,
+    apply nondet.program.falsify.mk,
+    { apply Te.enable },
+    { apply Te.schedule },
+    { apply Te.negate' } },
+end
+
+lemma local_reasoning.unless
+  (S : unless (s i) p q)
+: unless s' p q :=
+begin
+  unfold unless,
+  intros σ σ' STEP,
+  apply S,
+  unfold unitb.step has_safety.step step,
+  unfold unitb.step has_safety.step step s' compose at STEP,
+  unfold program.mch program.asm nondet.is_step nondet.program.lbl at STEP,
+  unfold nondet.program.step_of nondet.program.event at STEP,
+  admit
+end
+
+theorem leads_to.subst {p q}
+  (H : p ↦ q in s i)
+: p ↦ q in s' :=
+unitb.leads_to.subst id _ _
+(@local_reasoning.transient i) (@local_reasoning.unless i) H
+
+theorem often_imp_often.subst {p q}
+  (H : p >~> q in s i)
+: p >~> q in s' :=
+unitb.often_imp_often.subst id _ _
+(@local_reasoning.transient i) (@local_reasoning.unless i) H
+
+end
+end decomposition
